feat: add another List.find?_eq_some lemma (#5974)
Inspired by https://github.com/leanprover-community/mathlib4/pull/18593

src/Init/Data/List/Find.lean
@@ -206,7 +206,8 @@ theorem IsInfix.findSome?_eq_none {l₁ l₂ : List α} {f : α → Option β} (
 @[simp] theorem find?_eq_none : find? p l = none ↔ ∀ x ∈ l, ¬ p x := by
   induction l <;> simp [find?_cons]; split <;> simp [*]
 
-theorem find?_eq_some : xs.find? p = some b ↔ p b ∧ ∃ as bs, xs = as ++ b :: bs ∧ ∀ a ∈ as, !p a := by
+theorem find?_eq_some_iff_append :
+    xs.find? p = some b ↔ p b ∧ ∃ as bs, xs = as ++ b :: bs ∧ ∀ a ∈ as, !p a := by
   induction xs with
   | nil => simp
   | cons x xs ih =>
@@ -241,6 +242,9 @@ theorem find?_eq_some : xs.find? p = some b ↔ p b ∧ ∃ as bs, xs = as ++ b 
           refine ⟨as, ⟨⟨bs, ?_⟩, fun a m => h₂ a (mem_cons_of_mem _ m)⟩⟩
           cases h₁
           simp
+
+@[deprecated find?_eq_some_iff_append (since := "2024-11-06")]
+abbrev find?_eq_some := @find?_eq_some_iff_append
 
 @[simp]
 theorem find?_cons_eq_some : (a :: xs).find? p = some b ↔ (p a ∧ a = b) ∨ (!p a ∧ xs.find? p = some b) := by
@@ -347,7 +351,7 @@ theorem find?_flatten_eq_some {xs : List (List α)} {p : α → Bool} {a : α} :
     xs.flatten.find? p = some a ↔
       p a ∧ ∃ as ys zs bs, xs = as ++ (ys ++ a :: zs) :: bs ∧
         (∀ a ∈ as, ∀ x ∈ a, !p x) ∧ (∀ x ∈ ys, !p x) := by
-  rw [find?_eq_some]
+  rw [find?_eq_some_iff_append]
   constructor
   · rintro ⟨h, ⟨ys, zs, h₁, h₂⟩⟩
     refine ⟨h, ?_⟩
