src/Init/Data/List/Nat/Find.lean
@@ -9,6 +9,32 @@ import Init.Data.List.Find
 
 namespace List
 
+open Nat
+
+theorem find?_eq_some_iff_getElem {xs : List α} {p : α → Bool} {b : α} :
+    xs.find? p = some b ↔ p b ∧ ∃ i h, xs[i] = b ∧ ∀ j : Nat, (hj : j < i) → !p xs[j] := by
+  rw [find?_eq_some_iff_append]
+  simp only [Bool.not_eq_eq_eq_not, Bool.not_true, exists_and_right, and_congr_right_iff]
+  intro w
+  constructor
+  · rintro ⟨as, ⟨bs, rfl⟩, h⟩
+    refine ⟨as.length, ⟨?_, ?_, ?_⟩⟩
+    · simp only [length_append, length_cons]
+      refine Nat.lt_add_of_pos_right (zero_lt_succ bs.length)
+    · rw [getElem_append_right (Nat.le_refl as.length)]
+      simp
+    · intro j h'
+      rw [getElem_append_left h']
+      exact h _ (getElem_mem h')
+  · rintro ⟨i, h, rfl, h'⟩
+    refine ⟨xs.take i, ⟨xs.drop (i+1), ?_⟩, ?_⟩
+    · rw [getElem_cons_drop, take_append_drop]
+    · intro a m
+      rw [mem_take_iff_getElem] at m
+      obtain ⟨j, h, rfl⟩ := m
+      apply h'
+      omega
+
 theorem findIdx?_eq_some_le_of_findIdx?_eq_some {xs : List α} {p q : α → Bool} (w : ∀ x ∈ xs, p x → q x) {i : Nat}
     (h : xs.findIdx? p = some i) : ∃ j, j ≤ i ∧ xs.findIdx? q = some j := by
   simp only [findIdx?_eq_findSome?_enum] at h
